Change some methods in  module

src/Knapsack/Module.dfy
@@ -1,160 +1,170 @@
 //include "Implementation/Solution.dfy"
 
-module Q {
-    class Solution {
-        var priority : real
+abstract module Q {
+  class Solution {
+    var priority : real
 
-        ghost predicate Compare(other : Solution)
-            reads this, other
-        {
-           this.priority < other.priority 
-        }
+    ghost predicate Compare(other : Solution)
+      reads this, other
+    {
+      this.priority < other.priority
+    }
+  }
+
+  /*
+   The following priority queue is implemented with a williams heap (binary heap)
+  */
+  class PriorityQueue {
+    var arr : array<Solution>
+    var count : int  // current number of elements, if count == arr.Length, array must grow
+
+
+    constructor PriorityQueue(size: int)
+      //ensures this.Valid()
+    {
+      this.arr := new Solution[0];
+      this.count := 0;
     }
 
-    /*
-     The following priority queue is implemented with a williams heap (binary heap)
-    */
-    class PriorityQueue {
-        var arr : array<Solution>
-        var count : int  // current number of elements, if count == arr.Length, array must grow
 
+    /* Predicates */
 
-        constructor PriorityQueue(size: int)
-            //ensures this.IsHeap()
-        {
-            this.arr := new Solution[0];
-            this.count := 0;
-        }
-
-
-        /* Predicates */
-
-        /* Predicate: true if the array satisfies the heap property */
-        predicate IsHeap() 
-            reads this, this.arr, set i | 0 <= i < this.arr.Length :: arr[i]
-        {
-            && 0 <= this.count <= arr.Length
-            && (forall i | 0 < i < this.count :: this.arr[(i-1)/2].priority < this.arr[i].priority)
-        }
-
-        /* Predicate: true if the heap has no elements */
-        predicate IsEmpty()
-            reads this
-        {
-            this.count == 0
-        }
-
-
-
-        /* Methods */
-
-        /* Method: return the maximum capacity of the heap */
-        method Size() returns (s : int)
-        {
-            return this.arr.Length;
-        }
-
-
-        /* Method: returns the current number of elements in the heap */
-        method Count() returns (c : int)
-        {
-            return this.count;
-        }
-
-
-        /* Method: returns the element with the minimum priority in the heap */
-        method Min() returns (m : Solution)
-            requires 0 < this.count <= this.arr.Length <= this.arr.Length
-            requires this.IsHeap()
-        {
-            return this.arr[0];
-        }
-
-        
-        /* Method: inserts an element to the heap */
-        method Insert(node : Solution)
-            modifies this, this.arr
-            requires this.IsHeap()
-            //ensures this.IsHeap()
-        {
-            if (this.count == this.arr.Length) {
-                Grow(node);
-            }
-            this.count := this.count + 1;
-            this.Float();     
-        }
-
-
-        /* Method: duplicates space of the heap */
-        method Grow(x : Solution)
-            modifies this, this.arr
-            requires 0 <= this.count == this.arr.Length
-            ensures this.count == old(this.count) // the number of elements does not change in this method. The Method Insert increases it
-            ensures this.arr.Length > old(this.arr.Length) // the length of the array increases
-            ensures fresh(this.arr) // is new in memory
-            ensures this.arr[0..this.count] == old(this.arr[0..this.count]) // the elements that were already in the array are preserved
-
-        {
-            // allocate new memory
-            var aux: array<Solution> := new Solution[2 * this.arr.Length + 1] (_ => x);
-            
-            // copy
-            var i := 0;
-            while i < this.count
-                decreases this.count-i
-                invariant 0 <= i <= this.count <= this.arr.Length < aux.Length && this.count == old(this.count)
-                invariant aux[0..i] == this.arr[0..i]
-                invariant this.arr[0..this.count] == old(this.arr[0..this.count])
-            {
-                aux[i] := this.arr[i];
-                i := i + 1;
-            }
-            assert aux[0..this.count] == this.arr[0..this.count] == old(this.arr[0..this.count]);
-            //assert Seq.Rev(aux[0..size]) == Seq.Rev(list[0..size]) == Seq.Rev(old(list[0..size]));
-            this.arr := aux;
-            //assert Model() == Seq.Rev(aux[0..size]);
-        }
-
-
-        /* Method: moves the last inserted node upward in the heap until the heap property is restored */
-        method Float()
-            modifies this.arr
-            requires 0 < this.count <= this.arr.Length
-            requires forall i | 0 < i < this.count - 1 :: this.arr[(i-1)/2].priority <= this.arr[i].priority
-            ensures this.IsHeap()
-        // {
-        //     var j := this.count - 1;
-        //     while j > 0 && this.arr[(j-1)/2].priority > this.arr[j].priority
-        //         invariant 0 <= j <= this.count - 1 < this.arr.Length
-        //         invariant forall i | 0 < i < this.count :: i != j ==> this.arr[(i-1)/2].priority <= this.arr[i].priority
-        //     {
-        //         this.arr[(j-1)/2], this.arr[j] := this.arr[j], this.arr[(j-1)/2];
-        //         j := (j-1)/2;
-        //     }
-        // }
-        
-
-
-        /* Method: deletes the element with the minimum priority of the heap */
-        method DeleteMin()
-            modifies this, this.arr
-            requires this.IsHeap()
-            requires 0 < this.count
-            //ensures this.IsHeap()
-        {
-            this.arr[0] := this.arr[this.count - 1];
-            this.count := this.count - 1;
-            //Sink(0, this.count);
-        }
-
-
-        /* Method: moves a node downward in the heap until the heap property is restored */
-        method Sink(s : nat, l : nat)
-            modifies this.arr
-            requires 0 <= s <= l == this.count <= arr.Length
-            requires forall i | 0 < i < this.count && (i-1)/2 != s :: this.arr[(i-1)/2].priority <= this.arr[i].priority
-            ensures this.IsHeap()
-        
-
+    /* Predicate: true if the segment [x, y) of the array satisfies the heap property*/
+    predicate isHeap(x : int, y : int)
+      reads this, this.arr, set i | 0 <= i < this.arr.Length :: arr[i]
+    {
+      && 0 <= x <= y <= arr.Length
+      && (forall i | x < i < y :: this.arr[(i-1)/2].priority < this.arr[i].priority)
     }
+
+    /* Predicate: true if the array satisfies the heap property */
+    predicate Valid()
+      reads this, this.arr, set i | 0 <= i < this.arr.Length :: arr[i]
+    {
+      this.isHeap(0, this.count)
+    }
+
+
+    /* Predicate: true if the heap has no elements */
+    predicate IsEmpty()
+      reads this
+    {
+      this.count == 0
+    }
+
+
+
+    /* Methods */
+
+    /* Method: returns the current number of elements in the heap */
+    method Size() returns (c : int)
+    {
+      return this.count;
+    }
+
+
+    /* Method: returns the element with the minimum priority in the heap */
+    method Min() returns (m : Solution)
+      requires 0 < this.count <= this.arr.Length <= this.arr.Length
+      requires this.Valid()
+    {
+      return this.arr[0];
+    }
+
+
+    /* Method: inserts an element to the heap */
+    method Insert(node : Solution)
+      modifies this, this.arr
+      requires this.Valid()
+      //ensures this.Valid()
+    {
+
+      if (this.IsEmpty()) {
+        var aux: array<Solution> := new Solution[1][node];
+        this.arr := aux;
+      }
+      else if (this.count < this.arr.Length) { // array is not full
+        this.arr[this.count] := node;
+      }
+      else { // array is full
+        Grow();
+        this.arr[this.count] := node;
+      }
+      this.count := this.count + 1;
+      this.Float();      
+    }
+
+
+    /* Method: duplicates space of the heap */
+    method Grow()        
+      modifies this, this.arr
+      requires 0 < this.count == this.arr.Length
+      ensures this.count == old(this.count) // the number of elements does not change in this method. The Method Insert increases it
+      ensures this.arr.Length > old(this.arr.Length) // the length of the array increases
+      ensures fresh(this.arr) // is new in memory
+      ensures this.arr[0..this.count] == old(this.arr[0..this.count]) // the elements that were already in the array are preserved
+    {
+      // allocate new memory
+      var last := this.arr[this.count-1];
+      var aux: array<Solution> := new Solution[2 * this.arr.Length] (_ => last);
+
+      // copy
+      var i := 0;
+      while i < this.count
+        decreases this.count-i
+        invariant 0 <= i <= this.count <= this.arr.Length < aux.Length && this.count == old(this.count)
+        invariant aux[0..i] == this.arr[0..i]
+        invariant this.arr[0..this.count] == old(this.arr[0..this.count])
+      {
+        aux[i] := this.arr[i];
+        i := i + 1;
+      }
+      assert aux[0..this.count] == this.arr[0..this.count] == old(this.arr[0..this.count]);
+      //assert Seq.Rev(aux[0..size]) == Seq.Rev(list[0..size]) == Seq.Rev(old(list[0..size]));
+      this.arr := aux;
+      //assert Model() == Seq.Rev(aux[0..size]);
+    }
+
+
+    /* Method: moves the last inserted node upward in the heap until the heap property is restored */
+    method Float()
+      modifies this.arr
+      requires 0 < this.count <= this.arr.Length
+      requires forall i | 0 < i < this.count - 1 :: this.arr[(i-1)/2].priority <= this.arr[i].priority
+      ensures this.Valid()
+    // {
+    //     var j := this.count - 1;
+    //     while j > 0 && this.arr[(j-1)/2].priority > this.arr[j].priority
+    //         invariant 0 <= j <= this.count - 1 < this.arr.Length
+    //         invariant forall i | 0 < i < this.count :: i != j ==> this.arr[(i-1)/2].priority <= this.arr[i].priority
+    //     {
+    //         this.arr[(j-1)/2], this.arr[j] := this.arr[j], this.arr[(j-1)/2];
+    //         j := (j-1)/2;
+    //     }
+    // }
+
+
+
+    /* Method: deletes the element with the minimum priority of the heap */
+    method DeleteMin()
+      modifies this, this.arr
+      requires this.Valid()
+      requires 0 < this.count
+      //ensures this.Valid()
+    {
+      this.arr[0] := this.arr[this.count - 1];
+      this.count := this.count - 1;
+      //Sink(0, this.count);
+    }
+
+
+    /* Method: moves a node downward in the heap until the heap property is restored */
+    method Sink(s : nat, l : nat)
+      modifies this.arr
+      requires 0 <= s <= l == this.count <= arr.Length
+      requires forall i | 0 < i < this.count && (i-1)/2 != s :: this.arr[(i-1)/2].priority <= this.arr[i].priority
+      ensures this.Valid()
+
+
+  }
 }
